SigmaHCOLRewriting.v
@@ -90,70 +90,9 @@ Pre-condition:
 
    *)
 
-  Lemma cast_vector_operator_OK_OK: forall i0 i1 o0 o1 (v: vector A i1)
-                                      (op: vector A i0 → svector A o0)
-    ,
-      (i0 ≡ i1 /\ o0 ≡ o1) -> is_OK ((cast_vector_operator
-                                      i0 o0
-                                      i1 o1
-                                      (OK ∘ op)) v).
-  Proof.
-    intros.
-    destruct H as [Hi Ho].
-    rewrite <- Ho. clear o1 Ho.
-    revert op.
-    rewrite Hi. clear i0 Hi.
-    intros.
-
-    unfold compose.
-    set (e := (λ x : vector A i1, @OK (vector (option A) o0) (op x))).
-
-    assert(is_OK (e v)).
-    {
-      unfold e. simpl. trivial.
-    }
-    revert H.
-    generalize dependent e. clear op.
-    intros.
-
-    rename i1 into i.
-    rename o0 into o.
-    (* here we arrived to more generic form of the lemma, stating that is_OK property is preserved by 'cast_vector_operator *)
-
-    unfold cast_vector_operator.
-    destruct (eq_nat_dec o o), (eq_nat_dec i i); try congruence.
-
-    compute.
-    destruct e0.
-    dep_destruct e1.
-    auto.
-  Qed.
-
-  
-  Lemma cast_vector_operator_OK_elim: forall i o (v: vector A i)
-                                        (op: vector A i → svector A o)
-    ,
-      forall (t: svector A o),
-        ((cast_vector_operator
-            i o
-            i o
-            (OK ∘ op)) v) ≡ OK t -> op v ≡ t.
-  Proof.
-    intros i o v op t.
-    unfold cast_vector_operator.
-    destruct (eq_nat_dec i i); try congruence.
-    destruct (eq_nat_dec o o); try congruence.
-    compute.
-    dep_destruct e.
-    dep_destruct e0.
-    intros.
-    inversion H.
-    reflexivity.
-  Qed.
-   
   Lemma BinOpPre: forall o st
-                        (f:A->A->A) `{pF: !Proper ((=) ==> (=) ==> (=)) f}
-                        (x: svector A (o+o)),
+                    (f:A->A->A) `{pF: !Proper ((=) ==> (=) ==> (=)) f}
+                    (x: svector A (o+o)),
       svector_is_dense x -> 
       is_OK (evalSigmaHCOL st (SHOBinOp o f) x).
   Proof.
@@ -166,10 +105,10 @@ Pre-condition:
   Qed.
 
   Lemma BinOpPost: forall o st
-                        (f:A->A->A) `{pF: !Proper ((=) ==> (=) ==> (=)) f}
-                        (x: svector A (o+o)),
+                     (f:A->A->A) `{pF: !Proper ((=) ==> (=) ==> (=)) f}
+                     (x: svector A (o+o)),
       forall (v: svector A o),
-      (evalSigmaHCOL st (SHOBinOp o f) x ≡ OK v) -> svector_is_dense v.
+        (evalSigmaHCOL st (SHOBinOp o f) x ≡ OK v) -> svector_is_dense v.
   Proof.
     simpl.
     intros.
@@ -245,7 +184,7 @@ Pre-condition:
         destruct (Vbuild_spec _). simpl. rewrite e. clear e.
         unfold GathBackwardMap_Spec. 
         generalize (GathBackwardMap_Spec_obligation_1 i o nbase
-                                                                          nstride Hsnz HD) as gath_map_oc. intros.
+                                                      nstride Hsnz HD) as gath_map_oc. intros.
         unfold VnthIndexMapped.
         simpl.
         generalize (gath_map_oc n HY (nbase + n * nstride) eq_refl) as HX1. clear gath_map_oc.
@@ -255,129 +194,25 @@ Pre-condition:
       + congruence.
   Qed.
 
-
-  Lemma index_op_is_partial_map:
-    ∀ (i o : nat)
-      (x : svector A i),
-        ∀ (f_spec: index_function_spec i o),
-          Vforall (fun z => is_None z \/ Vin_aux x z)
-                  (vector_index_backward_operator f_spec x).
-      Proof.
-        intros.
-        unfold index_function_spec in f_spec.
-        unfold vector_index_backward_operator, proj1_sig,
-        vector_index_backward_operator_spec.
-        replace (let (a, _) :=
-                     Vbuild_spec (VnthIndexMapped x f_spec) in
-                 a) with
-        (Vbuild (VnthIndexMapped x f_spec)) by reflexivity.
-        apply Vforall_eq. intros.
-        apply Vbuild_in in H.
-        destruct H. destruct H. 
-        subst x0.
-        case_eq (VnthIndexMapped x f_spec x1 x2).
-        + right.
-          unfold VnthIndexMapped, proj1_sig in H.
-          destruct (f_spec x1 x2) in H.
-          destruct x0.
-          * rewrite <- H.
-            unfold Vin_aux.
-            apply Vnth_in.
-          * congruence.
-        + left.
-          none_some_elim.
-      Qed.
-
-  Lemma index_op_preserves_P:
-    ∀ (i o : nat) (x : svector A i) (P: option A->Prop),
-      P None ->
-      Vforall P x
-      → ∀ f_spec : index_function_spec i o,
-          Vforall P (vector_index_backward_operator f_spec x).
-  Proof.
-    intros.
-    unfold index_function_spec in f_spec.
-    assert(Vforall (fun z => is_None z \/ Vin_aux x z)
-                   (vector_index_backward_operator f_spec x))
-      by apply index_op_is_partial_map.
-    generalize dependent (vector_index_backward_operator f_spec x).
-    intros t.
-    rewrite 2!Vforall_eq.
-    crush.
-    assert (is_None x0 ∨ Vin_aux x x0) by (apply H1; assumption).
-    inversion H3.
-    + destruct x0; none_some_elim.
-      assumption.
-    + rewrite Vforall_eq in H0.
-      auto.
-  Qed.
-
-  Definition index_function_is_surjective
-             (i o : nat)
-             (f_spec: index_function_spec i o) :=
-    forall (j:nat) (jp:j<o), is_Some(proj1_sig (f_spec j jp)).
   
-  Lemma index_op_is_dense:
-    ∀ (i o : nat) (x : svector A i)
-      (f_spec: index_function_spec i o),
-      svector_is_dense x ->
-      index_function_is_surjective i o f_spec -> 
-      svector_is_dense (vector_index_backward_operator f_spec x).
-  Proof.
-    intros i o x f_spec xdense fsurj.
-    unfold index_function_spec in f_spec.
-    unfold index_function_is_surjective in fsurj.
-    unfold svector_is_dense in *.
-    unfold vector_index_backward_operator, proj1_sig,
-    vector_index_backward_operator_spec.
-    
-    replace (let (a, _) :=
-                 Vbuild_spec (VnthIndexMapped x f_spec) in
-             a) with
-    (Vbuild (VnthIndexMapped x f_spec)) by reflexivity.
-    apply Vforall_eq. intros.
-    apply Vbuild_in in H.
-    destruct H. destruct H. 
-    subst x0.
-    case_eq (VnthIndexMapped x f_spec x1 x2). 
-    - intros. 
-      none_some_elim.
-    - intros.
-      assert(FS: is_Some (` (f_spec x1 x2))) by apply fsurj.
-      unfold VnthIndexMapped, proj1_sig in H.
-      destruct (f_spec x1 x2) in H, FS; none_some_elim.
-      destruct x0.
-      +
-        simpl in *.
-        generalize dependent (l n eq_refl). 
-        clear FS f_spec fsurj l.
-        intros.
-        (* here we have a contradiction between 'xdense' and 'H' *)
-        assert (HS: is_Some (Vnth x l)) by (apply Vforall_nth; assumption).
-        destruct (Vnth x l); simpl in *;  congruence.
-      +
-        simpl in FS. contradiction FS.
-  Qed.
-
-
   (* Gath on dense vector produces dense vector *)
-
-    Lemma gath_math_surj:
-      ∀ (i o base stride : nat) (snz : 0 ≢ stride) (range_bound : base + pred o * stride < i),
-        index_function_is_surjective i o
-                                     (GathBackwardMap_Spec
-                                        (snz:=snz)
-                                        (range_bound:=range_bound)
-                                        i o base stride).
-    Proof.
-      unfold index_function_is_surjective.
-      simpl.
-      trivial.
-    Qed.
+  
+  Lemma gath_map_surj:
+    ∀ (i o base stride : nat) (snz : 0 ≢ stride) (range_bound : base + pred o * stride < i),
+      index_function_is_surjective i o
+                                   (GathBackwardMap_Spec
+                                      (snz:=snz)
+                                      (range_bound:=range_bound)
+                                      i o base stride).
+  Proof.
+    unfold index_function_is_surjective.
+    simpl.
+    trivial.
+  Qed.
   
   Lemma GathDensePost: forall (i o: nat) (base stride:aexp) (st:state)
-                           (y: svector A o)
-                           (x: svector A i),
+                         (y: svector A o)
+                         (x: svector A i),
       svector_is_dense x -> 
       (evalSigmaHCOL st (SHOGathH (i:=i) (o:=o) base stride) x) ≡ OK y ->
       svector_is_dense y.
@@ -393,7 +228,7 @@ Pre-condition:
     inversion 1.
     unfold GathH in *.
     apply index_op_is_dense; try assumption.
-    apply gath_math_surj.
+    apply gath_map_surj.
   Qed.
 
 
@@ -427,13 +262,13 @@ Pre-condition:
         (strideE: evalsToWithVar var st stride o)
         (xdense: svector_is_dense x):
     
-        evalSigmaHCOL st (SHOBinOp o f) x =
-        evalSigmaHCOL st (SHOISumUnion var (AConst o)
-                                       (SHOCompose _ _
-                                                   (SHOScatHUnion (AValue var) pad)
-                                                   (SHOCompose _ _ 
-                                                               (SHOBinOp 1 f)
-                                                               (SHOGathH (i:=o+o) (AValue var) stride)))) x.
+    evalSigmaHCOL st (SHOBinOp o f) x =
+    evalSigmaHCOL st (SHOISumUnion var (AConst o)
+                                   (SHOCompose _ _
+                                               (SHOScatHUnion (AValue var) pad)
+                                               (SHOCompose _ _ 
+                                                           (SHOBinOp 1 f)
+                                                           (SHOGathH (i:=o+o) (AValue var) stride)))) x.
   Proof.
     intros.
     unfold evalSigmaHCOL at 1.
@@ -468,7 +303,7 @@ Pre-condition:
       Focus 2. intros s C. rewrite C in bOK. err_ok_elim.
 
       intros.
- 
+      
       assert(sOK: is_OK (@evalScatHUnion A 1 1 (update st var 0) (AValue var) pad t0)).
       {
         apply ScatPre with (nbase:=0) (npad:=1).
@@ -489,7 +324,7 @@ Pre-condition:
 
   
   Definition ASub: A -> A -> A := (plus∘negate).
- 
+  
   Global Instance ASub_proper:
     Proper ((=) ==> (=) ==> (=)) (ASub).
   Proof.
@@ -510,67 +345,11 @@ Pre-condition:
                              (SHOCompose _ _ 
                                          (SHOBinOp 1 ASub)
                                          (SHOGathH (i:=4) (o:=2) vari c2))).
-
+  
   Lemma testOp2Op1: forall (st : state) (x : vector (option A) (2 + 2)),
       svector_is_dense x -> evalSigmaHCOL st op1 x = evalSigmaHCOL st op2 x.
   Proof.
-    intros.
-    unfold equiv, maybeError_equiv, op1.
-    assert (op1OK: is_OK (evalSigmaHCOL st (SHOBinOp 2 ASub) x)) by (apply BinOpPre; assumption). 
-
-    case_eq (evalSigmaHCOL st (SHOBinOp 2 ASub) x); intros; simpl in H0, op1OK.
-
-    Focus 2.
-    rewrite H0 in op1OK.
-    contradiction.
-
-    unfold op2, vari, c2, evalSigmaHCOL.
-    simpl.
-    
-    assert (g1OK: is_OK
-              (@evalGathH A Ae 4 2
-                          (update st (Var "i") 1)
-                          (AValue (Var "i"))
-                          (AConst 2) x)).
-    {
-      assert(g1_pre_nbase: evalAexp (update st (Var "i") 1) (AValue (Var "i")) ≡ OK 1).
-      {
-        simpl. unfold update.
-        destruct eq_varname_dec. reflexivity.
-        congruence.
-      }
-      
-      assert(g2_pre_nstride: evalAexp (update st (Var "i") 1) (AConst 2) ≡ OK 2).
-      {
-        simpl. unfold update.
-        reflexivity.
-      }
-      
-      apply GathPre with (nbase:=1) (nstride:=2) ; repeat (split; try assumption; try auto).
-    }
-
-    case_eq (@evalGathH A Ae 4 2 (update st (Var "i") 1) (AValue (Var "i"))
-                        (AConst 2) x); intros.
-    Focus 2.  rewrite H1 in g1OK. err_ok_elim.
-    apply GathDensePost in H1 ; try assumption.
-
-    assert(b1OK: is_OK (@evalBinOp A 2 1 (update st (Var "i") 1) ASub t0)).
-    {
-      apply BinOpPre.
-      apply ASub_proper.
-      assumption.
-    }
- 
-    case_eq (@evalBinOp A 2 1 (update st (Var "i") 1) ASub t0).
-    Focus 2. intros. rewrite H2 in b1OK. err_ok_elim.
-    intros.
-    apply BinOpPost in H0; try apply ASub_proper.
-
-
-    (* it looks like it could be proven this way but it is work intesive and stupid.
-        should be proven in generic form with variables instead of concrete values *)
-
-    
+    appy BinOpSums.
   Qed.
   
   Section SigmaHCOLRewriting.
